`iterable_expression.v`: attempt the first at defining a spec for packages

theories/approxis/examples/iterable_expression.v
@@ -36,24 +36,28 @@ Section motivating_example.
     
   End proofs.
 
-  (* Hence, the semantic typing assumption is not enough, we need something stronger *)
+  (* Hence, the semantic typing assumption is not enough,
+    we need something stronger *)
 End motivating_example.
 
 Section defs.
 
-  Fixpoint ForallSep {Σ} {A} (P : A → iProp Σ) (l : list A) : (iProp Σ) := match l with
+  Fixpoint ForallSep {Σ} {A} (P : A → iProp Σ)
+    (l : list A) : (iProp Σ) := match l with
     | [] => True
     | h :: t => P h ∗ (ForallSep P t)
   end.
 
-  Fixpoint ForallSep2 {Σ A B} (P : A → B → iProp Σ) (l1 : list A) (l2 : list B) : (iProp Σ) :=
+  Fixpoint ForallSep2 {Σ A B} (P : A → B → iProp Σ)
+    (l1 : list A) (l2 : list B) : (iProp Σ) :=
   match l1, l2 with
     | [], [] => True
     | h1 :: t1, h2 :: t2 => P h1 h2 ∗ (ForallSep2 P t1 t2)
     | _, _ => False
   end.
 
-  Fixpoint ForallSep3 {Σ A B C} (P : A → B → C → iProp Σ) (l1 : list A) (l2 : list B) (l3 : list C) : (iProp Σ) :=
+  Fixpoint ForallSep3 {Σ A B C} (P : A → B → C → iProp Σ)
+    (l1 : list A) (l2 : list B) (l3 : list C) : (iProp Σ) :=
   match l1, l2, l3 with
     | [], [], [] => True
     | h1 :: t1, h2 :: t2, h3 :: t3 => P h1 h2 h3 ∗ (ForallSep3 P t1 t2 t3)
@@ -103,14 +107,17 @@ Section rules.
   Section deterministic.
 
     (*
-    Definition det_val_fun {A : Type} {As : list Type} (f : expr) (f_sem : list val -> val)
+    Definition det_val_fun {A : Type} {As : list Type}
+      (f : expr) (f_sem : list val -> val)
       (types : list (lrel Σ)) : Prop :=
       ∀ (E : coPset)
       (K : list (ectxi_language.ectx_item prob_ectxi_lang))
       (args : list val) (e : expr) (A : lrel Σ),
       ForallSep2 (fun x T => (lrel_car T) x x) args types ⊢
-      (refines E (fill K (f_sem args)) e A -∗ refines E (fill K (iter_appl_expr f args)) e A) ∧
-      (refines E e (fill K (f_sem args)) A -∗ refines E e (fill K (iter_appl_expr f args)) A).
+      (refines E (fill K (f_sem args)) e A -∗
+        refines E (fill K (iter_appl_expr f args)) e A) ∧
+      (refines E e (fill K (f_sem args)) A -∗
+        refines E e (fill K (iter_appl_expr f args)) A).
     *)
     
     (* Check [nat : Type] : list Type. *)(*
@@ -123,14 +130,16 @@ Section rules.
       (K : list (ectxi_language.ectx_item prob_ectxi_lang))
       (args : ∀ A, A ∈ As → A) (e : expr) (A : lrel Σ),
       ForallSep2 (λ A Arel, ∀ x : A,
-          (lrel_car Arel) ((inject (to_vals A _)) x) ((inject (to_vals A _)) x)) As rel_types
+          (lrel_car Arel)
+          ((inject (to_vals A _)) x) ((inject (to_vals A _)) x))As rel_types
       ⊢ True.
       (refines E (fill K (to_val (fold_right (λ f x, f x) f_sem args))) e A
         -∗ refines E (fill K (iter_appl_expr f args)) e A) ∧
       (refines E e (fill K (to_val (fold_right (λ f x, f x) f_sem args))) A
         -∗ refines E e (fill K (iter_appl_expr f args)) A).*)
 
-    Definition to_val_type_rel {A : Type} (Arel : lrel Σ) (to_val : A → val) : iProp Σ :=
+    Definition to_val_type_rel {A : Type}
+      (Arel : lrel Σ) (to_val : A → val) : iProp Σ :=
       ∀ x : A, (lrel_car Arel) (to_val x) (to_val x).
 
     Definition det_val_fun1 {A B : Type} (Alrel Blrel : lrel Σ)
@@ -153,8 +162,10 @@ Section rules.
       (K : list (ectxi_language.ectx_item prob_ectxi_lang))
       (args : list val) (e : expr) (A : lrel Σ),
       ForallSep2 (fun x T => (lrel_car T) x x) args types ⊢
-      (refines E (fill K (f_sem args)) e A -∗ refines E (fill K (iter_appl_expr f args)) e A) ∧
-      (refines E e (fill K (f_sem args)) A -∗ refines E e (fill K (iter_appl_expr f args)) A).
+      (refines E (fill K (f_sem args)) e A -∗
+        refines E (fill K (iter_appl_expr f args)) e A) ∧
+      (refines E e (fill K (f_sem args)) A -∗
+        refines E e (fill K (iter_appl_expr f args)) A).
 
     Definition det_val_rel (f : expr) (types : list (lrel Σ)) : Prop :=
       ∀ (E : coPset)
@@ -162,8 +173,10 @@ Section rules.
       (args : list val) (e : expr) (A : lrel Σ),
       ForallSep2 (fun x T => (lrel_car T) x x) args types ⊢
       ∃ (v : val),
-      (refines E (fill K v) e A -∗ refines E (fill K (iter_appl_expr f args)) e A) ∧
-      (refines E e (fill K v) A -∗ refines E e (fill K (iter_appl_expr f args)) A).
+      (refines E (fill K v) e A -∗
+        refines E (fill K (iter_appl_expr f args)) e A) ∧
+      (refines E e (fill K v) A -∗
+        refines E e (fill K (iter_appl_expr f args)) A).
     
     Theorem det_val_fun_rel : forall e f_sem types, det_val_fun e f_sem types ->
       det_val_rel e types.
@@ -217,10 +230,12 @@ Section rules.
       (K : list (ectxi_language.ectx_item prob_ectxi_lang))
       (n : Z) (e : expr) (A : lrel Σ), ∃ (v : val),
       ((∀ (ll : list loc) (lv : list val),
-        ⌜length ll = Nref⌝ -∗ ForallSep2 (fun l v => l ↦ v) ll lv -∗ (refines E (fill K v) e A))
+        ⌜length ll = Nref⌝ -∗ ForallSep2 (fun l v => l ↦ v) ll lv -∗
+          (refines E (fill K v) e A))
       ⊢ (refines E (fill K (f #n)) e A)) ∧
       ((∀ (ll : list loc) (lv : list val),
-        ⌜length ll = Nref⌝ -∗ ForallSep2 (fun l v => l ↦ₛ v) ll lv -∗ (refines E e (fill K v) A))
+        ⌜length ll = Nref⌝ -∗ ForallSep2 (fun l v => l ↦ₛ v) ll lv -∗
+          (refines E e (fill K v) A))
       ⊢ (refines E e (fill K (f #n)) A)).
 
     Definition val2 : val :=
@@ -263,7 +278,8 @@ Section rules.
         (e' : expr) (B : lrel Σ),
           (refines E' e' (fill K' v) B) -∗ (refines E' e' (fill K' (f #n)) B)).
 
-    Definition couplable (f : list loc -> val) (C : lrel Σ) (lN : list nat) : Prop :=
+    Definition couplable (f : list loc -> val)
+      (C : lrel Σ) (lN : list nat) : Prop :=
       ∀ (E : coPset)
       (K : list (ectxi_language.ectx_item prob_ectxi_lang))
       (n : Z) (e : list loc -> expr) (A : lrel Σ) (lιl lιr : list loc),
@@ -287,7 +303,8 @@ Section rules.
       iMod "Hec".
       destruct lιl as [|hιl tιl]; last destruct tιl as [|hιl' tιl];
       destruct lιr as [|hιr tιr]; try destruct tιr as [|hιr' tιr]; simpl;
-      try done; try (iDestruct "Hι" as "[_ Hι]"; done); try (iDestruct "Hι'" as "[_ Hι']"; done).
+      try done; try (iDestruct "Hι" as "[_ Hι]"; done);
+        try (iDestruct "Hι'" as "[_ Hι']"; done).
       iDestruct "Hι" as "[Hι _]"; iDestruct "Hι'" as "[Hι' _]".
       rel_apply (refines_couple_TT_err 10 10); try lia.
       { Unshelve. 6:{ exact 0%R. } 1: { lra. } all: shelve. }
@@ -326,7 +343,8 @@ Section rules.
     end.
 
   Lemma lazy_eager' (li li' : list loc) :
-    ForallSep2 (fun i n => i ↪N (n;[])) li l ∗ ForallSep2 (fun i n => i ↪ₛN (n;[])) li' l
+    ForallSep2 (fun i n => i ↪N (n;[])) li l ∗
+      ForallSep2 (fun i n => i ↪ₛN (n;[])) li' l
     ⊢ REL (eager_exec' li) << lazy_exec'  li' : () → lrel_int.
   Proof with rel_pures_l; rel_pures_r. rewrite /eager_exec'. iIntros "[Hi Hi']".
     rel_bind_l (foo' _ _).
@@ -346,7 +364,8 @@ Section rules.
     iIntros (v1 v2 [eq1 eq2]); subst.
     rel_apply refines_na_inv; iSplitL; first iAssumption.
     iIntros "[[[Hx Hpotential]|Hx] Hclose]";
-    replace (0)%Z with (Z.of_nat 0)%Z by lia; rel_pures_l; rel_pures_r; rel_load_r...
+    replace (0)%Z with (Z.of_nat 0)%Z by lia;
+    rel_pures_l; rel_pures_r; rel_load_r...
     - rel_apply "Hpotential"...
       rel_store_r... rel_apply refines_na_close; iFrame.
       rel_values.
@@ -367,4 +386,188 @@ Section rules.
     iFrame.
   Qed.
 
-End rules.
+  Section package.
+    (* Attempt to formalize a well-formed package,
+      that may initialize some references, tapes, etc
+      before providing several functions *)
+
+    (*
+      A package is:
+      - An expression `package`, possibly with side effects, reducing
+        to a value `package_initialized` (this reduction is the
+        _initialization_ of the package) together with
+      - getters; a given getter, let's say `getter_i`,
+        applied to `package_initialized`, reduces to
+        a value `f_i` such that
+      - under some assumptions, provide a value having
+        some properties, that need to be declared with
+        the package.
+      - Additionally, even though a package can take account
+        for locations declared during the initialization, it
+        doesn't track (for now) new locations allocated
+        during the execution of a `f_i`.
+        E.g.
+        ```
+        let: "x" := ref 0 in
+        (λ: <>, !"x", λ: <>, incr "x")
+        ```
+        corresponds perfectly to a package where the class will
+        be useful, but the class won't be able to correctly
+        encompass the behavior of the following program:
+        ```
+        let: "x" := ref 0 in
+        (λ: <>, !"x", λ: <>, let "y" := ref 0 in incr "x")
+        ```
+    *)
+
+    Context `{!approxisRGS Σ}.
+
+    Definition ForallIndex {A : Type} (P : nat → A → Prop) (l : list A) : Prop :=
+      (fix ForallIndexAux (A : Type) i P (l : list A) : Prop :=
+        match l with
+          | [] => True
+          | [a] => P i a
+          | a :: (_ :: _) as t => P i a ∧ ForallIndexAux A (S i) P t
+        end) A 0 P l.
+    
+    Definition ForallIndex2 {A B : Type} (P : nat → A → B → Prop)
+      (l1 : list A) (l2 : list B) : Prop :=
+      (fix ForallIndexAux2 (A B : Type) i P (l1 : list A) (l2 : list B) : Prop :=
+        match l1, l2 with
+          | [], [] => True
+          | [a], [b] => P i a b
+          | a :: (_ :: _) as t1, b :: (_ :: _) as t2
+            => P i a b ∧ ForallIndexAux2 A B (S i) P t1 t2
+          | _, _ => False
+        end) A B 0 P l1 l2.
+    
+    Definition ForallIndex3 {A B C : Type} (P : nat → A → B → C → Prop)
+      (l1 : list A) (l2 : list B) (l3 : list C) : Prop :=
+      (fix ForallIndexAux3 (A B C : Type) i P
+        (l1 : list A) (l2 : list B) (l3 : list C) : Prop :=
+        match l1, l2, l3 with
+          | [], [], [] => True
+          | [a], [b], [c] => P i a b c
+          | a :: (_ :: _) as t1, b :: (_ :: _) as t2, c :: (_ :: _) as t3
+            => P i a b c ∧ ForallIndexAux3 A B C (S i) P t1 t2 t3
+          | _, _, _ => False
+        end) A B C 0 P l1 l2 l3.
+
+    Fixpoint list_full_of {X} (n : nat) (x : X) : list X := match n with
+      | S n' => x :: list_full_of n' x
+      | O => []
+    end.
+
+    (* [n_0, ..., n_(i-1), ...] ~~> [n_0, ...,n_(i-1) + 1, ...]*)
+    Fixpoint next_package_state (i : nat) (ns : list nat) : list nat :=
+      match i, ns with
+        | _, [] => []
+        | O, h :: t => (S h) :: t
+        | S i', h :: t => h :: (next_package_state i' t)
+      end.
+
+    Definition package_function_spec
+      {P_l P_r : list nat → list loc → iProp Σ}
+      {P_lr : list nat → list nat → list loc → list loc → iProp Σ}
+      {R_l R_r : list nat → list val → val → iProp Σ}
+      {lls rls : list loc}
+      (lrel_args : list (lrel Σ)) (lrel_return : lrel Σ)
+      (method : list loc → val) (i : nat) : Prop :=
+        ∀ (args : list val),
+            (* left execution *)
+            ∀ (ns : list nat) K e E (A : lrel Σ),
+              Forall2 (λ arg t, ⊢ (lrel_car t) arg arg) args lrel_args →
+              (P_l ns lls ⊢
+                (∃ v,
+                  (R_l ns args v ∗ P_l (next_package_state i ns) lls
+                    -∗ refines E (fill K (Val v)) e A)
+                  -∗ refines E (fill K (iter_appl_expr (method lls) args)) e A))
+            (* right execution *)
+          ∧ ∀ (ms : list nat) K e E (A : lrel Σ),
+              Forall2 (λ arg t, ⊢ (lrel_car t) arg arg) args lrel_args →
+              (P_r ms rls ⊢
+                (∃ v,
+                  (R_r ms args v ∗ P_l (next_package_state i ms) rls
+                    -∗ refines E e (fill K (Val v)) A)
+                  -∗ refines E e (fill K (iter_appl_expr (method rls) args)) A))
+            (* for an execution on both sides, we can use
+              a semantic typing assumption *)
+          ∧ ∀ (ns ms : list nat) (𝒩 : namespace) (P : iProp Σ),
+              (∃ Q, P ⊣⊢ (P_lr ns ms lls rls) ∗ Q) →
+              (na_invP 𝒩 P
+              ⊢ refines top (method lls) (method rls)
+                (fold_right (λ A B : lrel Σ, (A → B)%lrel) lrel_return lrel_args)).
+
+    Definition initialized_package
+      {P_l P_r : list nat → list loc → iProp Σ}
+      {P_lr : list nat → list nat → list loc → list loc → iProp Σ}
+      {R_l R_r : list nat → list val → val → iProp Σ}
+      (lrel_car_argss : list (list (lrel Σ))) (lrel_car_returns : list (lrel Σ))
+      (lls rls : list loc) (getters : list val) (package_initialized : list loc → val) :=
+      @ForallIndex3 val (list (lrel Σ)) (lrel Σ)
+        (λ i getter lrel_car_args lrel_car_return,
+          (∃ (method : list loc → val),
+          (* A getter provides a value v... *)
+              (∀ K e E A,
+                 (refines E (fill K (Val (method lls))) e A
+                ⊢ refines E (fill K (getter (package_initialized lls))) e A)
+              ∧  (refines E e (fill K (method rls)) A
+                ⊢ refines E e (fill K (getter (package_initialized rls))) A))
+              ∧ @package_function_spec P_l P_r P_lr R_l R_r
+                  lls rls lrel_car_args lrel_car_return method i))
+        getters lrel_car_argss lrel_car_returns.
+    
+    Class PACKAGE_PARAMS (N_functions : nat) (*(N_loc : nat)*) := {
+        n_arg : list nat
+      ; n_arg_len : length n_arg = N_functions
+      ; P_l   : list nat → list loc → iProp Σ
+        (* property on the LHS, needed and obtained
+          by running one of the values of the package *)
+      ; P_r   : list nat → list loc → iProp Σ
+        (* idem, on the RHS *)
+      ; P_lr  : list nat → list nat → list loc → list loc → iProp Σ
+      ; P_rem : list nat → list nat → list loc → list loc → iProp Σ
+      (* properties got on the return value of each method *)
+      ; Rval_l : list nat → list val → val → iProp Σ
+      ; Rval_r : list nat → list val → val → iProp Σ
+        (* to replace with semantic type of each method*)
+      ; Plr_l_r : ∀ ns ms lls rls,
+          P_lr ns ms lls rls ⊣⊢
+          P_l ns lls ∗ P_r ms rls ∗ P_rem ns ms lls rls : Prop
+        (* ...then I wonder if P_lr is really needed *)
+    }.
+
+    Class PACKAGE_STRUCT (N_functions : nat) := {
+        package : expr
+      ; getters : list val
+      ; len_getters : length getters = N_functions
+    }.
+
+    Class PACKAGE `{package_struct : !PACKAGE_STRUCT N_functions}
+      {package_params : PACKAGE_PARAMS N_functions} := {
+        lrel_car_return : list (lrel Σ)
+      ; lrel_car_args : list (list (lrel Σ))
+      ; lrel_car_args_len : Forall2 (λ lrel_args n_args,
+        length lrel_args = n_args) lrel_car_args n_arg
+      ; rel_init : ⊢ (∀ K e E A,
+          ∃ (package_initialized : list loc → val) (lls rls : list loc),
+              P_l (list_full_of N_functions 0) lls
+            ∗ P_r (list_full_of N_functions 0) rls
+            ∗ ⌜@initialized_package
+                P_l P_r P_lr
+                Rval_l Rval_r
+                lrel_car_args lrel_car_return
+                lls rls
+                getters package_initialized⌝
+            ∗  ⌜refines E (fill K (Val (package_initialized lls))) e A
+              ⊢ refines E (fill K package) e A⌝
+            ∧  ⌜refines E e (fill K (Val (package_initialized rls))) A
+              ⊢ refines E e (fill K package) A⌝)%I
+    }.
+
+    Lemma package_getter_valid_index `{!PACKAGE_STRUCT n} {i : nat} (Hltin : i < n)
+      : i < length getters.
+    Proof. rewrite len_getters. apply Hltin. Qed.
+  End package.
+
+End rules.  
